language/move-prover/tests/sources/functional/emits.move
@@ -1,0 +1,80 @@
+module TestEmits {
+    use 0x1::Event::{Self, EventHandle};
+
+    struct DummyEvent {
+        msg: u64
+    }
+
+    // -------------------------
+    // simple `emits` statements
+    // -------------------------
+
+    public fun simple(handle: &mut EventHandle<DummyEvent>) {
+        Event::emit_event(handle, DummyEvent{msg: 0});
+    }
+    spec fun simple {
+        emits DummyEvent{msg: 0} to handle;
+    }
+
+    public fun simple_wrong_msg_incorrect(handle: &mut EventHandle<DummyEvent>) {
+        Event::emit_event(handle, DummyEvent{msg: 0});
+    }
+    spec fun simple_wrong_msg_incorrect {
+        emits DummyEvent{msg: 1} to handle;
+    }
+
+    public fun simple_wrong_handle_incorrect(handle: &mut EventHandle<DummyEvent>, _handle2: &mut EventHandle<DummyEvent>) {
+        Event::emit_event(handle, DummyEvent{msg: 0});
+    }
+    spec fun simple_wrong_handle_incorrect {
+        emits DummyEvent{msg: 0} to _handle2;
+    }
+
+
+    // ------------------------------
+    // conditional `emits` statements
+    // ------------------------------
+
+    public fun conditional(x: u64, handle: &mut EventHandle<DummyEvent>) {
+        if (x > 7) {
+            Event::emit_event(handle, DummyEvent{msg: 0});
+        }
+    }
+    spec fun conditional {
+        emits DummyEvent{msg: 0} to handle if x > 7;
+    }
+
+    public fun conditional_wrong_condition_incorrect(x: u64, handle: &mut EventHandle<DummyEvent>) {
+        if (x > 7) {
+            Event::emit_event(handle, DummyEvent{msg: 0});
+        }
+    }
+    spec fun conditional_wrong_condition_incorrect {
+        emits DummyEvent{msg: 0} to handle if x > 0;
+    }
+
+    public fun conditional_missing_condition_incorrect(x: u64, handle: &mut EventHandle<DummyEvent>) {
+        if (x > 7) {
+            Event::emit_event(handle, DummyEvent{msg: 0});
+        }
+    }
+    spec fun conditional_missing_condition_incorrect {
+        emits DummyEvent{msg: 0} to handle;
+    }
+
+
+    // ----------------------------
+    // `emits` statements in schema
+    // ----------------------------
+
+    public fun emits_in_schema(handle: &mut EventHandle<DummyEvent>) {
+        Event::emit_event(handle, DummyEvent{msg: 0});
+    }
+    spec fun emits_in_schema {
+        include EmitsInSchemaEmits;
+    }
+    spec schema EmitsInSchemaEmits {
+        handle: EventHandle<DummyEvent>;
+        emits DummyEvent{msg: 0} to handle;
+    }
+}
